src/language_extension.lean
@@ -1,4 +1,4 @@
-import .fol tactic.tidy
+import tactic.tidy .compactness
 
 open set function nat
 universe variable u
@@ -9,28 +9,36 @@ local notation `[` l:(foldr `, ` (h t, dvector.cons h t) dvector.nil `]`:0) := l
 
 
 namespace Language
+def Lconstants (α : Type u) : Language :=
+⟨λn, nat.rec α (λn ih, pempty) n, λn, pempty⟩
+
 protected def sum (L L' : Language) : Language :=
 ⟨λn, L.functions n ⊕ L'.functions n, λ n, L.relations n ⊕ L'.relations n⟩
 
 def symbols (L : Language) := (Σl, L.functions l) ⊕ (Σl, L.relations l)
 end Language
 
--- section
--- variable {L : Language}
+section
+variable {L : Language}
 
 
--- def symbols_in_term : ∀{l}, preterm L l → set L.symbols
--- | _ &k          := ∅
--- | l (func f)    := {sum.inl ⟨l,f⟩}
--- | _ (app t₁ t₂) := symbols_in_term t₁ ∪ symbols_in_term t₂
+def symbols_in_term : ∀{l}, preterm L l → set L.symbols
+| _ &k          := ∅
+| l (func f)    := {sum.inl ⟨l,f⟩}
+| _ (app t₁ t₂) := symbols_in_term t₁ ∪ symbols_in_term t₂
 
--- def symbols_in_formula : ∀{l}, preformula L l → set L.symbols
--- | _ falsum       := ∅
--- | _ (t₁ ≃ t₂)    := symbols_in_term t₁ ∪ symbols_in_term t₂
--- | l (rel R)      := {sum.inr ⟨l, R⟩}
--- | _ (apprel f t) := symbols_in_formula f ∪ symbols_in_term t
--- | _ (f₁ ⟹ f₂)   := symbols_in_formula f₁ ∪ symbols_in_formula f₂
--- | _ (∀' f)       := symbols_in_formula f
+def symbols_in_formula : ∀{l}, preformula L l → set L.symbols
+| _ falsum       := ∅
+| _ (t₁ ≃ t₂)    := symbols_in_term t₁ ∪ symbols_in_term t₂
+| l (rel R)      := {sum.inr ⟨l, R⟩}
+| _ (apprel f t) := symbols_in_formula f ∪ symbols_in_term t
+| _ (f₁ ⟹ f₂)   := symbols_in_formula f₁ ∪ symbols_in_formula f₂
+| _ (∀' f)       := symbols_in_formula f
+
+def symbols_in_formula_subst (s : term L) : ∀{l} (n) (f : preformula L l), 
+  symbols_in_formula (f[s // n]) ⊆ symbols_in_formula f ∪ symbols_in_term s := sorry
+
+end
 
 -- def symbols_in_prf : ∀{Γ : set $ formula L} {f : formula L} (P : Γ ⊢ f), set L.symbols
 -- | Γ f (axm h)              := symbols_in_formula f
@@ -51,7 +59,6 @@ end Language
   
 
 
--- end
 
 structure Lhom (L L' : Language) :=
 (on_function : ∀{n}, L.functions n → L'.functions n) 
@@ -65,6 +72,12 @@ variables {L : Language.{u}} {L' : Language.{u}} (ϕ : L →ᴸ L')
 
 protected def id (L : Language) : L →ᴸ L :=
 ⟨λn, id, λ n, id⟩
+
+protected def sum_inl {L L' : Language} : L →ᴸ L.sum L' :=
+⟨λn, sum.inl, λ n, sum.inl⟩
+
+protected def sum_inr {L L' : Language} : L' →ᴸ L.sum L' :=
+⟨λn, sum.inr, λ n, sum.inr⟩
 
 @[reducible]def comp {L1} {L2} {L3} (g : L2 →ᴸ L3) (f : L1 →ᴸ L2) : L1 →ᴸ L3 :=
 begin
@@ -97,6 +110,10 @@ class has_decidable_range : Type u :=
 
 attribute [instance] has_decidable_range.on_function has_decidable_range.on_relation
 
+@[simp] def on_symbol : L.symbols → L'.symbols
+| (sum.inl ⟨l, f⟩) := sum.inl ⟨l, ϕ.on_function f⟩
+| (sum.inr ⟨l, R⟩) := sum.inr ⟨l, ϕ.on_relation R⟩
+
 @[simp] def on_term : ∀{l}, preterm L l → preterm L' l
 | _ &k          := &k
 | _ (func f)    := func $ ϕ.on_function f
@@ -121,6 +138,13 @@ attribute [instance] has_decidable_range.on_function has_decidable_range.on_rela
   ϕ.on_term (apps t ts) = apps (ϕ.on_term t) (ts.map ϕ.on_term)
 | _ t []       := by refl
 | _ t (t'::ts) := by simp*
+
+lemma not_mem_symbols_in_term_on_term {s : L'.symbols} (h : s ∉ range (ϕ.on_symbol)) :
+  ∀{l} (t : preterm L l), s ∉ symbols_in_term (ϕ.on_term t)
+| _ &k          := not_mem_empty _
+| l (func f)    := λh', h ⟨sum.inl ⟨l, f⟩, (eq_of_mem_singleton h').symm⟩
+| _ (app t₁ t₂) := 
+  λh, or.elim h (not_mem_symbols_in_term_on_term t₁) (not_mem_symbols_in_term_on_term t₂)
 
 @[simp] def on_formula : ∀{l}, preformula L l → preformula L' l
 | _ falsum       := falsum
@@ -156,6 +180,19 @@ attribute [instance] has_decidable_range.on_function has_decidable_range.on_rela
   ϕ.on_formula (apps_rel f ts) = apps_rel (ϕ.on_formula f) (ts.map ϕ.on_term)
 | _ f []       := by refl
 | _ f (t'::ts) := by simp*
+
+lemma not_mem_symbols_in_formula_on_formula {s : L'.symbols} (h : s ∉ range (ϕ.on_symbol)) :
+  ∀{l} (f : preformula L l), s ∉ symbols_in_formula (ϕ.on_formula f) := sorry
+
+lemma not_mem_function_in_formula_on_formula {l'} {f' : L'.functions l'} 
+  (h : f' ∉ range (@on_function _ _ ϕ l')) {l} (f : preformula L l) :
+  (sum.inl ⟨l', f'⟩ : L'.symbols) ∉ symbols_in_formula (ϕ.on_formula f) :=
+begin
+  apply not_mem_symbols_in_formula_on_formula,
+  intro h', apply h, 
+  rcases h' with ⟨⟨n, f⟩ | ⟨n, R⟩, hf₂⟩; dsimp at hf₂; cases hf₂ with hf₂',
+  apply mem_range_self
+end
 
 @[simp] def on_bounded_term {n} : ∀{l} (t : bounded_preterm L n l), bounded_preterm L' n l
 | _ &k           := &k
@@ -257,6 +294,8 @@ lemma id_bounded_formula {L} : Π n l, Π f, (@on_bounded_formula L L (Lhom.id L
 
 @[simp] def on_closed_term (t : closed_term L) : closed_term L' := ϕ.on_bounded_term t
 @[simp] def on_sentence (f : sentence L) : sentence L' := ϕ.on_bounded_formula f
+def on_sentence_fst (f : sentence L) : (ϕ.on_sentence f).fst = ϕ.on_formula f.fst :=
+ϕ.on_bounded_formula_fst f
 
 def on_prf {Γ : set $ formula L} {f : formula L} (h : Γ ⊢ f) : ϕ.on_formula '' Γ ⊢ ϕ.on_formula f :=
 begin
@@ -293,12 +332,22 @@ begin
   refine (term.elim_apps _ _ f ts).trans _, rw [dif_pos hf], refl
 end
 
-lemma reflect_term_apps_neg [has_decidable_range ϕ] {l} (f : L'.functions l) 
+lemma reflect_term_apps_neg [has_decidable_range ϕ] {l} {f : L'.functions l} 
   (hf : f ∉ range (@on_function _ _ ϕ l)) (ts : dvector (term L') l) (m : ℕ) : 
   ϕ.reflect_term (apps (func f) ts) m = &m :=
 begin
   refine (term.elim_apps _ _ f ts).trans _, rw [dif_neg hf]
 end
+
+lemma reflect_term_const_pos [has_decidable_range ϕ] {c : L'.constants}
+  (hf : c ∈ range (@on_function _ _ ϕ 0)) (m : ℕ) : 
+  ϕ.reflect_term (func c) m = func (classical.some hf) :=
+by apply reflect_term_apps_pos hf ([]) m
+
+lemma reflect_term_const_neg [has_decidable_range ϕ] {c : L'.constants}
+  (hf : c ∉ range (@on_function _ _ ϕ 0)) (m : ℕ) : 
+  ϕ.reflect_term (func c) m = &m :=
+by apply reflect_term_apps_neg hf ([]) m
 
 @[simp] lemma reflect_term_var [has_decidable_range ϕ] (k : ℕ) (m : ℕ) : 
   ϕ.reflect_term &k m = &k ↑' 1 # m := by refl
@@ -380,10 +429,10 @@ by simp [reflect_formula, formula.rec_apps_rel, dif_neg hR]
 @[simp] lemma reflect_formula_all [has_decidable_range ϕ] (f : formula L') (m : ℕ) : 
   ϕ.reflect_formula (∀' f) m = ∀' (ϕ.reflect_formula f (m+1)) := by refl
 
-@[simp] lemma reflect_formula_on_formula [has_decidable_range ϕ] (hϕ : is_injective ϕ) 
-  (f : formula L) : ∀(m : ℕ), ϕ.reflect_formula (ϕ.on_formula f) m = f ↑' 1 # m :=
+@[simp] lemma reflect_formula_on_formula [has_decidable_range ϕ] (hϕ : is_injective ϕ) (m : ℕ)
+  (f : formula L) : ϕ.reflect_formula (ϕ.on_formula f) m = f ↑' 1 # m :=
 begin
-  refine formula.rec _ _ _ _ _ f; clear f; intros,
+  revert m, refine formula.rec _ _ _ _ _ f; clear f; intros,
   { refl },
   { simp [hϕ] },
   { simp [reflect_formula_apps_rel_pos (mem_range_self R), hϕ], 
@@ -447,6 +496,103 @@ begin
   { apply subst, have h := @H_ih_h₁ m, simp at h, exact h,
     have h := @H_ih_h₂ m, simp [hϕ] at h, exact h, simp [hϕ] },
 end
+
+section 
+
+/- maybe generalize to filter_symbol? -/
+@[reducible] def filter_symbols (p : L.symbols → Prop) : Language :=
+⟨λl, subtype (λf, p (sum.inl ⟨l, f⟩)), λl, subtype (λR, p (sum.inr ⟨l, R⟩))⟩
+
+def filter_symbols_Lhom (p : L.symbols → Prop) : filter_symbols p →ᴸ L :=
+⟨λl, subtype.val, λl, subtype.val⟩
+
+def is_injective_filter_symbols_Lhom (p : L.symbols → Prop) : 
+  is_injective (filter_symbols_Lhom p) :=
+⟨λl, subtype.val_injective, λl, subtype.val_injective⟩
+
+lemma find_term_filter_symbols (p : L.symbols → Prop) : 
+  ∀{l} (t : preterm L l) (h : symbols_in_term t ⊆ { s | p s }), 
+  { t' : preterm (filter_symbols p) l // (filter_symbols_Lhom p).on_term t' = t }
+| _ &k          h := ⟨&k, rfl⟩
+| _ (func f)    h := ⟨func ⟨f, h $ mem_singleton _⟩, rfl⟩ 
+| _ (app t₁ t₂) h := 
+  begin
+    let ih₁ := find_term_filter_symbols t₁ (subset.trans (subset_union_left _ _) h),
+    let ih₂ := find_term_filter_symbols t₂ (subset.trans (subset_union_right _ _) h),
+    refine ⟨app ih₁.1 ih₂.1, _⟩, dsimp, rw [ih₁.2, ih₂.2]
+  end
+
+lemma find_formula_filter_symbols (p : L.symbols → Prop) : 
+  ∀{l} (f : preformula L l) (h : symbols_in_formula f ⊆ { s | p s }), 
+  { f' : preformula (filter_symbols p) l // (filter_symbols_Lhom p).on_formula f' = f }
+| _ falsum       h := ⟨⊥, rfl⟩
+| _ (t₁ ≃ t₂)    h :=
+  begin
+    let ih₁ := find_term_filter_symbols p t₁ (subset.trans (subset_union_left _ _) h),
+    let ih₂ := find_term_filter_symbols p t₂ (subset.trans (subset_union_right _ _) h),
+    refine ⟨ih₁.1 ≃ ih₂.1, _⟩, dsimp, rw [ih₁.2, ih₂.2]
+  end
+| _ (rel R)      h := ⟨rel ⟨R, h $ mem_singleton _⟩, rfl⟩ 
+| _ (apprel f t) h :=
+  begin
+    let ih₁ := find_formula_filter_symbols f (subset.trans (subset_union_left _ _) h),
+    let ih₂ := find_term_filter_symbols p t (subset.trans (subset_union_right _ _) h),
+    refine ⟨apprel ih₁.1 ih₂.1, _⟩, dsimp, rw [ih₁.2, ih₂.2]
+  end
+| _ (f₁ ⟹ f₂)   h :=
+  begin
+    let ih₁ := find_formula_filter_symbols f₁ (subset.trans (subset_union_left _ _) h),
+    let ih₂ := find_formula_filter_symbols f₂ (subset.trans (subset_union_right _ _) h),
+    refine ⟨ih₁.1 ⟹ ih₂.1, _⟩, dsimp, rw [ih₁.2, ih₂.2]
+  end
+| _ (∀' f)       h := 
+  begin
+    let ih := find_formula_filter_symbols f h,
+    refine ⟨∀' ih.1, _⟩, dsimp, rw [ih.2]
+  end
+
+end
+
+noncomputable def generalize_constant {Γ} (c : L.constants)
+  (hΓ : (sum.inl ⟨0, c⟩ : L.symbols) ∉ ⋃₀ (symbols_in_formula '' Γ))
+  {f : formula L} (hf : (sum.inl ⟨0, c⟩ : L.symbols) ∉ symbols_in_formula f)
+  (H : Γ ⊢ f[func c // 0]) : Γ ⊢ ∀' f :=
+begin
+  apply allI,
+  let p : L.symbols → Prop := (≠ sum.inl ⟨0, c⟩),
+  let ϕ := filter_symbols_Lhom p,
+  have hϕ : is_injective ϕ := is_injective_filter_symbols_Lhom p,
+  have hc : c ∉ range (on_function ϕ),
+  { intro hc, rw [mem_range] at hc, rcases hc with ⟨c', hc'⟩, 
+    apply c'.2, rw [←hc'], refl },
+  have hf' : symbols_in_formula f ⊆ {s : Language.symbols L | p s},
+  { intros s hs hps, subst hps, exact hf hs },
+  rcases find_formula_filter_symbols p f hf' with ⟨f, rfl⟩,
+  have : {Γ' // Lhom.on_formula ϕ '' Γ' = Γ } ,
+  { refine ⟨Lhom.on_formula ϕ ⁻¹' Γ, _⟩,
+    apply image_preimage_eq_of_subset, intros f' hf',
+    have : symbols_in_formula f' ⊆ {s : Language.symbols L | p s},
+    { intros s hs hps, subst hps, exact hΓ ⟨_, mem_image_of_mem _ hf', hs⟩ },
+    rcases find_formula_filter_symbols p f' this with ⟨f, rfl⟩, 
+    apply mem_range_self },
+  rcases this with ⟨Γ, rfl⟩,
+  rw [image_image, ←image_congr' (ϕ.on_formula_lift 1), 
+    ←image_image ϕ.on_formula], 
+  apply ϕ.on_prf,
+  haveI : has_decidable_range (filter_symbols_Lhom p) := 
+    ⟨λn f, classical.prop_decidable _, λn R, classical.prop_decidable _⟩,
+  have := reflect_prf_gen hϕ 0 H,
+  rwa [reflect_formula_subst0 hϕ, reflect_term_const_neg hc, image_image,
+    image_congr' (reflect_formula_on_formula hϕ 0), 
+    reflect_formula_on_formula hϕ, lift_subst_formula_cancel] at this  
+end
+
+noncomputable def sgeneralize_constant {T : Theory L} (c : L.constants)
+  (hΓ : (sum.inl ⟨0, c⟩ : L.symbols) ∉ ⋃₀ (symbols_in_formula '' T.fst))
+  {f : bounded_formula L 1} (hf : (sum.inl ⟨0, c⟩ : L.symbols) ∉ symbols_in_formula f.fst)
+  (H : T ⊢ f[bd_func c /0]) : T ⊢ ∀' f :=
+by { simp [sprf] at H, exact generalize_constant c hΓ hf H }
+
 
 noncomputable def reflect_prf {Γ : set $ formula L} {f : formula L} (hϕ : ϕ.is_injective)
   (h : ϕ.on_formula '' Γ ⊢ ϕ.on_formula f) : Γ ⊢ f :=
@@ -549,6 +695,46 @@ variable {ϕ}
 lemma is_consistent_Theory_induced (hϕ : ϕ.is_injective) {T : Theory L} (hT : is_consistent T) : 
   is_consistent (ϕ.Theory_induced T) :=
 λH, hT $ H.map $ λh, reflect_sprf hϕ (by apply h)
+
+/- we could generalize this, replacing set.univ by any set s, but then we cannot use set.image
+  anymore (since the domain of g would be s), and things would be more annoying -/
+def is_consistent_extend {T : Theory L} (hT : is_consistent T) (hϕ : ϕ.is_injective)
+  (h : bounded_formula L 1 → bounded_formula L 1)
+  (hT' : ∀(f : bounded_formula L 1), T ⊢ ∃' (h f))
+  (g : bounded_formula L 1 → L'.constants) (hg : injective g) 
+  (hg' : ∀x, g x ∉ range (@on_function L L' ϕ 0)) : 
+  is_consistent (ϕ.Theory_induced T ∪ 
+  (λf, (ϕ.on_bounded_formula (h f))[bd_const (g f)/0]) '' set.univ) :=
+begin
+  haveI : decidable_eq (bounded_formula L 1) := λx y, classical.prop_decidable _,
+  haveI : decidable_eq (sentence L') := λx y, classical.prop_decidable _,
+  have lem : ∀(s₀ : finset (bounded_formula L 1)), 
+    is_consistent (ϕ.Theory_induced T ∪ 
+      (λf, (ϕ.on_bounded_formula (h f))[bd_const (g f)/0]) '' ↑s₀),
+  { refine finset.induction _ _,
+    { simp, exact is_consistent_Theory_induced hϕ hT },
+    { intros ψ s hψ ih hs, refine sprovable.elim _ hs, clear hs, intro hs, apply ih, constructor,
+      simp [image_insert_eq] at hs,
+      have : _ ⊢ (ϕ.on_bounded_formula $ ∼(h ψ))[bd_const (g ψ)/0] := simpI hs,
+      have := sgeneralize_constant (g ψ) _ _ this,
+      { refine simpE _ _ this, apply sweakening (subset_union_left _ _) (ϕ.on_sprf $ hT' ψ) },
+      { intro h', rcases h' with ⟨s', ⟨ψ', ⟨ψ', ⟨ψ', hψ₂, rfl⟩ | ⟨ψ', hψ₂, rfl⟩, rfl⟩, rfl⟩, hψ₃⟩, 
+        { rw [ϕ.on_sentence_fst] at hψ₃, 
+          exact ϕ.not_mem_function_in_formula_on_formula (hg' _) _ hψ₃ },
+        { simp at hψ₃, 
+          cases symbols_in_formula_subst _ _ _ hψ₃ with hψ₄ hψ₄,
+          { exact ϕ.not_mem_function_in_formula_on_formula (hg' _) _ hψ₄ },
+          { injection eq_of_mem_singleton hψ₄ with hψ₅, injection hψ₅ with x hψ₆, 
+            cases hg (eq_of_heq hψ₆), exact hψ hψ₂ }}},
+      { rw [on_bounded_formula_fst], apply not_mem_function_in_formula_on_formula, apply hg' }}},
+  intro H, rcases theory_proof_compactness H with ⟨T₀, h₀, hT⟩,
+  have : decidable_pred (∈ ϕ.Theory_induced T) := λx, classical.prop_decidable _,
+  rcases finset.subset_union_elim hT with ⟨t₀, s₀, rfl, ht₀, hs₀⟩,
+  have hs₀' := subset.trans hs₀ (diff_subset _ _),
+  rcases finset.exists_of_subset_image hs₀' with ⟨s₀, hs₀x, rfl⟩,
+  apply lem s₀, refine h₀.map _, apply sweakening,
+  simp, refine subset.trans ht₀ _, simp
+end
 
 end Lhom
 
